first level corrections

FirstLevel.v
@@ -6,11 +6,31 @@ Module Type FirstLevel (Import coh: Coherence) (Import cl: CacheLocal coh).
   Definition clean a t p :=
     le Sh (state a t p) /\ forall c, parent c p -> le (dir a t p c) Sh.
 
-  About noStore.
+  Print noStore.
 
   Definition noStoreData a d t :=
     d = initData a /\ forall t', t' < t -> noStore a (respFn a) t'.
 
+  Definition isStoreData a d t :=
+    exists tm, tm < t /\ match respFn a tm with
+                           | Some (Build_Resp cm im dm) =>
+                             let (descQm, dtQm) := reqFn a cm im in
+                             d = dtQm /\ descQm = St /\
+                             forall t', tm < t' < t -> noStore a (respFn a) t'
+                           | None => False
+                         end.
+  Parameter latestValue:
+    forall a t pCache,
+      let p := node pCache in
+      clean a t p ->
+      noStoreData a (data a t p) t \/ isStoreData a (data a t p) t.
+
+  Parameter processReq:
+    forall a t, 
+      match respFn a t with
+        | Some (Build_Resp cProc _ _) =>
+          let c := p_node cProc in
+          let (op, d) := reqFn a cProc (next a t c) in
           match op with
             | Ld => le Sh (state a t c)
             | St => state a t c = Mo
@@ -42,27 +62,26 @@ Module mkStoreAtomic (Import coh: Coherence) (Import cl: CacheLocal coh) (Import
     Variable a: Addr.
     Lemma nextIncOrSame:
       forall t p,
-        let c := p_node p in
-        next a t c = next a (S t) c \/
-        next a (S t) c = S (next a t c).
+        next a (S t) (p_node p) = next a t (p_node p) \/
+        next a (S t) (p_node p) = S (next a t (p_node p)).
     Proof.
-      intros t p c.
-      assert (opts: next a t c = next a (S t) c \/
-                    next a (S t) c <> next a t c) by omega.
+      intros t p.
+      assert (opts: next a (S t) (p_node p) = next a t (p_node p) \/
+                    next a (S t) (p_node p) <> next a t (p_node p)) by omega.
       pose proof (@nextChange a t p) as nextChange.
       pose proof (noReqAgain a t) as noReqAgain.
       destruct opts; repeat destructAll;
       try match goal with
-            | [H: (next (S t) c <> next t c) |- _ ] =>
-                specialize (nextChange H); try rewrite nextChange in *
+            | [H: (next a (S t) (p_node p) <> next a t (p_node p)) |- _ ] =>
+                specialize (nextChange H); try rewrite <- nextChange in *
           end;
       intuition.
     Qed.
 
     Lemma increasingIdx: forall t1 t2, t1 <= t2 -> forall p,
                                                      let c := p_node p in
-                                                     next t1 c <=
-                                                     next t2 c.
+                                                     next a t1 c <=
+                                                     next a t2 c.
     Proof.
       intros t1 t2 cond p c.
       diff t1 t2 cond.
@@ -71,17 +90,17 @@ Module mkStoreAtomic (Import coh: Coherence) (Import cl: CacheLocal coh) (Import
       destruct (nextIncOrSame (t1 + td) p) as [eq|neq]; unfold c in *; omega.
     Qed.
 
-    Lemma incrOnResp: forall t1 t2, t1 < t2 -> match respFn t1 with
+    Lemma incrOnResp: forall t1 t2, t1 < t2 -> match respFn a t1 with
                                                  | Some (Build_Resp c1 i1 _) =>
-                                                   next t2 (p_node c1) > i1
+                                                   next a t2 (p_node c1) > i1
                                                  | _ => True
                                                end.
     Proof.
       intros t1 t2 t1_lt_t2.
       assert (St1_le_t2: S t1 <= t2) by omega.
       pose proof (increasingIdx St1_le_t2) as u1.
-      pose proof (noReqAgain t1).
-      pose proof (respFnIdx t1).
+      pose proof (noReqAgain a t1).
+      pose proof (respFnIdx a t1).
       repeat destructAll;
         repeat match goal with
           | c: Proc |- _ => specialize (u1 c); omega
@@ -90,7 +109,7 @@ Module mkStoreAtomic (Import coh: Coherence) (Import cl: CacheLocal coh) (Import
     Qed.
 
     Theorem uniqRespLabels':
-      forall t1 t2, match respFn t1, respFn t2 with
+      forall t1 t2, match respFn a t1, respFn a t2 with
                       | Some (Build_Resp c1 i1 _), Some (Build_Resp c2 i2 _) =>
                         p_node c1 = p_node c2 -> i1 = i2 -> t1 = t2
                       | _, _ => True
@@ -98,7 +117,7 @@ Module mkStoreAtomic (Import coh: Coherence) (Import cl: CacheLocal coh) (Import
     Proof.
       Ltac finish incrOnResp respFnIdx t2 slt :=
         specialize (incrOnResp _ _ slt);
-        specialize (respFnIdx t2);
+        specialize (respFnIdx a t2);
         repeat destructAll;
         match goal with
           | _ => intros pEq idEq; rewrite pEq, idEq in *; omega
@@ -115,7 +134,7 @@ Module mkStoreAtomic (Import coh: Coherence) (Import cl: CacheLocal coh) (Import
     Qed.
 
     Theorem localOrdering':
-      forall t1 t2, match respFn t1, respFn t2 with
+      forall t1 t2, match respFn a t1, respFn a t2 with
                       | Some (Build_Resp c1 i1 _), Some (Build_Resp c2 i2 _) =>
                         p_node c1 = p_node c2 -> i1 > i2 -> t1 > t2
                       | _, _ => True
@@ -126,8 +145,8 @@ Module mkStoreAtomic (Import coh: Coherence) (Import cl: CacheLocal coh) (Import
       destruct opts as [lt|le].
       repeat destructAll; intuition.
       pose proof (increasingIdx le) as incr.
-      pose proof (respFnIdx t1) as r1.
-      pose proof (respFnIdx t2) as r2.
+      pose proof (respFnIdx a t1) as r1.
+      pose proof (respFnIdx a t2) as r2.
       repeat destructAll; intros;
         repeat match goal with
                  | [H: p_node ?p1 = p_node ?p2 |- _] =>
@@ -140,9 +159,9 @@ Module mkStoreAtomic (Import coh: Coherence) (Import cl: CacheLocal coh) (Import
     Lemma allPrevIdx:
       forall t2 p2 i1,
         let c2 := p_node p2 in
-        i1 < next t2 c2 ->
+        i1 < next a t2 c2 ->
         exists t1, t1 < t2 /\
-                   match respFn t1 with
+                   match respFn a t1 with
                      | Some (Build_Resp c1 i _) =>
                          p_node c1 = c2 /\ i = i1
                      | None => False
@@ -163,15 +182,15 @@ Module mkStoreAtomic (Import coh: Coherence) (Import cl: CacheLocal coh) (Import
       rewrite same in *.
       finishPrev IHt2 t2 i1LtNext.
 
-      assert (opts: i1 < next t2 (p_node p2) \/ i1 = next t2 (p_node p2))
+      assert (opts: i1 < next a t2 (p_node p2) \/ i1 = next a t2 (p_node p2))
              by omega;
       destruct opts as [lt | same].
       finishPrev IHt2 t2 lt.
 
       rewrite same in *.
-      assert (ne: next (S t2) (p_node p2) <> next t2 (p_node p2)) by omega.
+      assert (ne: next a (S t2) (p_node p2) <> next a t2 (p_node p2)) by omega.
       pose proof (nextChange p2 ne).
-      pose proof (respFnIdx t2).
+      pose proof (respFnIdx a t2).
       exists t2.
       repeat destructAll; try omega; match goal with
                                        | [H: p_node ?p = p_node p2 |- _ ] => rewrite <- H in *; intuition
@@ -179,10 +198,10 @@ Module mkStoreAtomic (Import coh: Coherence) (Import cl: CacheLocal coh) (Import
     Qed.
 
     Theorem allPrevious':
-      forall t2, match respFn t2 with
+      forall t2, match respFn a t2 with
                    | Some (Build_Resp c2 i2 _) =>
                        forall i1, i1 < i2 -> exists t1, t1 < t2 /\
-                                                           match respFn t1 with
+                                                           match respFn a t1 with
                                                              | Some (Build_Resp c1 i _) =>
                                                                  p_node c1 = p_node c2 /\ i = i1
                                                              | None => False
@@ -192,15 +211,13 @@ Module mkStoreAtomic (Import coh: Coherence) (Import cl: CacheLocal coh) (Import
     Proof.
       intros t2.
       pose proof (@allPrevIdx t2) as u1.
-      pose proof (respFnIdx t2).
+      pose proof (respFnIdx a t2).
       repeat destructAll;
       try match goal with
             | [p: Proc |- _] => specialize (u1 (p_node p))
           end; intuition.
     Qed.
-  End ForAddr.
 
-  Section Sa.
     Lemma leafProp: forall p c, ~ parent c (node (proc p)).
     Proof.
       unfold not; intros p c c_p.
@@ -211,11 +228,11 @@ Module mkStoreAtomic (Import coh: Coherence) (Import cl: CacheLocal coh) (Import
     Qed.
 
     Lemma cleanProp:
-      forall t p loc,
-        le Sh (state t (node (proc p)) loc) ->
-        le Sh (state t (node (proc p)) loc) /\
+      forall t p,
+        le Sh (state a t (node (proc p))) ->
+        le Sh (state a t (node (proc p))) /\
         (forall c, parent c (node (proc p)) ->
-                   le (dir t (node (proc p)) c loc) Sh).
+                   le (dir a t (node (proc p)) c) Sh).
     Proof.
       intros.
       pose proof (leafProp p) as leafProp.
@@ -228,12 +245,12 @@ Module mkStoreAtomic (Import coh: Coherence) (Import cl: CacheLocal coh) (Import
 
     Theorem storeAtomicity':
       forall t,
-        match respFn t with
+        match respFn a t with
           | Some (Build_Resp c i d) =>
-            let (a, descQ, dtQ) := reqFn c i in
+            let (descQ, dtQ) := reqFn a c i in
             match descQ with
               | Ld =>
-                  noStoreData d a t \/ isStoreData d a t
+                  noStoreData a d t \/ isStoreData a d t
               | St => d = initData zero
             end
           | _ => True
@@ -242,10 +259,10 @@ Module mkStoreAtomic (Import coh: Coherence) (Import cl: CacheLocal coh) (Import
       intros t.
       unfold noStoreData, isStoreData.
       pose proof (@cleanProp t) as cleanProp.
-      pose proof (respFnIdx t) as respFnIdx.
-      pose proof (respFnLdData t) as respFnLdData.
-      pose proof (@latestValue t).
-      pose proof (processReq t) as processReq.
+      pose proof (respFnIdx a t) as respFnIdx.
+      pose proof (respFnLdData a t) as respFnLdData.
+      pose proof (@latestValue a t).
+      pose proof (processReq a t) as processReq.
       unfold p_node in *.
       destructAll.
       destructAll.
@@ -253,7 +270,7 @@ Module mkStoreAtomic (Import coh: Coherence) (Import cl: CacheLocal coh) (Import
       destructAll.
       destructAll.
 
-      specialize (latestValue (proc procR) (cleanProp _ _ processReq));
+      specialize (latestValue (proc procR) (cleanProp _ processReq));
       simpl in *; rewrite <- respFnLdData in *;
       intuition.
 
@@ -262,10 +279,10 @@ Module mkStoreAtomic (Import coh: Coherence) (Import cl: CacheLocal coh) (Import
       intuition.
     Qed.
 
-    Theorem fullStoreAtomicity: StoreAtomicity respFn.
+    Theorem fullStoreAtomicity: StoreAtomicity a (respFn a).
     Proof.
-      apply (Build_StoreAtomicity respFn uniqRespLabels' localOrdering'
+      apply (Build_StoreAtomicity a (respFn a) uniqRespLabels' localOrdering'
                                   allPrevious' storeAtomicity').
     Qed.
-  End Sa.
+  End ForAddr.
 End mkStoreAtomic.
